---
mathLink: auto
---

<div class="topSpace"></div>

Date Created: 10/06/2023 13:39:14
Tags: #Type/Proposition #Topic/Number_Theory

Proved by: [[Fundamental Theorem of Arithmetic]], [[Chinese Remainder Theorem]]
References: <i>Not Applicable</i>
Justifications: <i>Not Applicable</i>

Specializations: <i>Not Applicable</i>
Generalizations: <i>Not Applicable</i>

``` ad-Proposition
title: Proposition.

For all $n\in\N^+$, we have $\phi\l(n\r)=n\prod_{p\divides n}\!\l(1-\frac{1}{p}\r)$.

```

<i>Proof.</i> Decompose $n=\prod p_i^{r_i}$ as a product of primes and note that $p_i^{r_i}\perp p_j^{r_j}$ for all $i\neq j$. Thus the ideals generated by $p_i^{r_i}$ and $p_j^{r_j}$ are coprime in $\Z$ for all $i\neq j$, and since $\gen{n}=\prod\gen{p_i^{r_i}}$, we see by the Chinese Remainder Theorem that $\Z/n\Z\iso\prod\Z/p_i^{r_i}\Z$. This induces an isomorphism $\l(\Z/n\Z\r)^\times\!\iso\prod\l(\Z/p_i^{r_i}\Z\r)^\times$, so, simply equating orders, we get $\phi\l(n\r)=\prod\phi\l(p_i^{r_i}\r)$. It remains to show that $\phi\l(p^r\r)=\l(p-1\r)p^{r-1}$ for all primes $p$ and $r\geq1$, whence
$$\begin{equation}
    \phi\l(n\r)=\prod\l(p_i-1\r)p_i^{r_i-1}=\prod p_i^{r_i}\l(1-\frac{1}{p_i}\r)=n\prod_{p\divides n}\l(1-\frac{1}{p}\r).
\end{equation}$$
* We prove $\phi\l(p^r\r)=\l(p-1\r)p^{r-1}=p^r-p^{r-1}$ by a counting argument. Indeed, for all $1\leq q\leq p^r$, $q$ and $p^r$ are coprime iff $\gcd\l(q,p^r\r)=1$, which occurs iff $q$ is not a multiple of $p$. There are $p^{r-1}$ multiples of $p$ ranging from $1$ to $p^r$, inclusive, so $m$ can take on ($p^r-p^{r-1}$)-many values.<span style="float:right;">$\blacksquare$</span>
